WIP: trying to prove export does not change behavior

IOHist.fst
@@ -60,11 +60,8 @@ let rec iohist_interpretation #a
 
 type set_of_traces = events_trace -> Type0
 
-val include_in : events_trace -> (set_of_traces) -> Type0
-let include_in t set = set t
-
-val subset : set_of_traces -> set_of_traces -> Type0
-let subset s1 s2 = forall t. s1 t ==>  s2 t
+val include_in : set_of_traces -> set_of_traces -> Type0
+let include_in s1 s2 = forall t. s1 t ==>  s2 t
 
 let rec behavior #a
   (m : io a) : set_of_traces =
@@ -76,15 +73,14 @@ let rec behavior #a
     | Call cmd args fnc -> (fun t' -> 
       (exists res t. (
          FStar.WellFounded.axiom1 fnc res;
-         ((include_in t (behavior (fnc res))) /\
-         t' == ((convert_call_to_event cmd args res)::t)))))
+         (behavior (fnc res) t) /\
+         t' == ((convert_call_to_event cmd args res)::t))))
   end
 
 let l : events_trace = []
 #set-options "--max_fuel 20 --max_ifuel 20"
-let _ = assert (include_in [EOpenfile "asdf" (Inl 7)] (behavior (Cont (Call Openfile "asdf" (fun x -> Return x))))) by (
+let _ = assert ((behavior (Cont (Call Openfile "asdf" (fun x -> Return x))) [EOpenfile "asdf" (Inl 7)])) by (
   unfold_def (`behavior);
-  unfold_def (`include_in);
   unfold_def (`convert_call_to_event);
   witness (`(Inl 7));
   witness (`l);
@@ -97,10 +93,9 @@ let code1 : io (res Close) =
 
 
 exception OneExc
-let _ = assert (include_in [EOpenfile "asdf" (Inr OneExc)] (behavior code1)) by (
+let _ = assert (behavior code1 [EOpenfile "asdf" (Inr OneExc)]) by (
   unfold_def (`code1);
   unfold_def (`behavior);
-  unfold_def (`include_in);
   unfold_def (`convert_call_to_event);
   witness (`(Inr OneExc));
   witness (`l);
@@ -143,14 +138,14 @@ let _ = assert (behavior' (Cont (Call Openfile "asdf" (fun x -> Return x))) (fun
   explode ();
   dump "h")
 
-let _ = assert (behavior' code1 (fun trace -> trace == [EOpenfile "asdf" (Inr OneExc)])) by (
-  unfold_def (`code1);
-  unfold_def (`behavior');
-  unfold_def (`convert_call_to_event);
-  witness (`(Inr OneExc));
-  witness (`l);
-  compute ();
-  dump "h")
+// let _ = assert (behavior' code1 (fun trace -> trace == [EOpenfile "asdf" (Inr OneExc)])) by (
+//   unfold_def (`code1);
+//   unfold_def (`behavior');
+//   unfold_def (`convert_call_to_event);
+//   witness (`(Inr OneExc));
+//   witness (`l);
+//   compute ();
+//   dump "h")
 
 (* total *)
 (* reifiable *)
